hybrid/Proof.lean
@@ -1,64 +1,93 @@
 import Hybrid.Form
 
--- Axiom utils. Since we won't be assuming a transitive frame,
--- it will make sense to be able to construct formulas with
--- iterated modal operators at their beginning (ex., for axiom nom)
-def iterate_nec (n : Nat) (φ : Form) : Form :=
-  let rec loop : Nat → Form → Form
-    | 0, φ   => φ
-    | n+1, φ => □ (loop n φ)
-  loop n φ
+section Tautology
+/-
+  def morphism_false {α : Type} (f : Form → set α) : Prop := ∀ a : α, (a ∈ f ⊥) → False 
+  def morphism_impl  {α : Type} (f : Form → set α) : Prop := ∀ (a : α) (φ ψ : Form), (a ∈ f (φ ⟶ ψ)) ↔ ((a ∈ f φ) → (a ∈ f ψ))
+  def Morphism {α : Type} (f : Form → set α) : Prop := (morphism_false f) ∧ (morphism_impl f)
+  def Tautology (φ : Form) : Prop := ∀ {α : Type} (f : Form → set α) (_ : Morphism f) (a : α), a ∈ f φ
+  
+  theorem test {φ ψ : Form} : Tautology (φ ⟶ (ψ ⟶ φ)) := by
+    intro α f ⟨_, impl⟩ a
+    rw [impl, impl]
+    intro h _
+    exact h
+-/
 
-def iterate_pos (n : Nat) (φ : Form) : Form :=
-  let rec loop : Nat → Form → Form
-    | 0, φ   => φ
-    | n+1, φ => ◇ (loop n φ)
-  loop n φ
+  class Morphism {α : Type} (f : Form → set α) where
+    morph_false : ∀ a : α, (a ∈ f ⊥) ↔ False
+    morph_impl  : ∀ (a : α) (φ ψ : Form), (a ∈ f (φ ⟶ ψ)) ↔ ((a ∈ f φ) → (a ∈ f ψ))
 
-inductive Proof (Γ : set Form) : Form → Type where
+  attribute [simp] Morphism.morph_false
+  attribute [simp] Morphism.morph_impl
+  @[simp]
+  def morph_neg {α : Type} (a : α) (f : Form → set α) [m : Morphism f] {φ : Form} : (a ∈ f (∼φ)) ↔ ((a ∈ f φ) → False) := by
+    simp
+  @[simp]
+  def morph_conj {α : Type} (a : α) (f : Form → set α) [m : Morphism f] {φ ψ : Form} : (a ∈ f (φ ⋀ ψ)) ↔ ((a ∈ f φ) ∧ (a ∈ f ψ)) := by
+    simp
+  @[simp]
+  def morph_disj {α : Type} (a : α) (f : Form → set α) [m : Morphism f] {φ ψ : Form} : (a ∈ f (φ ⋁ ψ)) ↔ ((a ∈ f φ) ∨ (a ∈ f ψ)) := by
+    simp
+
+  def Tautology (φ : Form) : Prop := ∀ {α : Type} (f : Form → set α) [Morphism f] (a : α), a ∈ f φ
+
+  theorem test {φ ψ : Form} : Tautology (φ ⟶ (ψ ⟶ φ)) := by
+    intro α f m a
+    rw [m.morph_impl, m.morph_impl]
+    intro h _
+    exact h
+
+end Tautology
+
+inductive Proof : set Form → Form → Type where
   -- Deduction rules:
   -- all premises (elements of Γ) can be deduced from Γ
-  | premise {φ : Form}:
+  | premise {Γ : set Form} {φ : Form}:
         (φ ∈ Γ) → Proof Γ φ
 
   -- if φ can be deduced from Γ, then so can ∀ v, φ
   -- todo: add restrictions 
-  | general {φ : Form} {t : SVAR} {v : SVAR}:
-        Proof Γ φ → Proof Γ (all v, φ) 
+  | general {Γ : set Form} {φ : Form} (v t : SVAR)
+      (restrict₁ : ∀ ψ : Form, ((ψ ∈ Γ) → occurs t ψ = false))
+      (restrict₂ : occurs v φ = false):    -- (restrict₂ : is_substable φ v t):
+        Proof Γ φ → Proof Γ (all v, φ[v // t]) 
 
-  -- if φ can be deduced from Γ, then so can □ φ
-  | necess {φ : Form}:
-        Proof Γ φ → Proof Γ (□ φ)
+  -- if φ is a theorem, □ φ can be deduced from any Γ 
+  | necess {Γ : set Form} {φ : Form}:
+        (∀ Δ : set Form, Proof Δ φ) → Proof Γ (□ φ)
 
   -- modus ponens:
-  | ponens {φ ψ : Form}:
+  | ponens {Γ : set Form} {φ ψ : Form}:
         Proof Γ (φ ⟶ ψ) → Proof Γ φ → Proof Γ ψ
 
   -- add all instances of propositional tautologies...
+  | tautology {Γ : set Form} {φ : Form}:
+        Tautology φ → Proof Γ φ
 
   -- Axioms for modal + hybrid logic:
   -- distribution schema (axiom K)
-  | ax_k {φ ψ : Form}:
+  | ax_k {Γ : set Form} {φ ψ : Form}:
         Proof Γ (□ (φ ⟶ ψ) ⟶ (□ φ ⟶ □ ψ))
 
-  | ax_q1 {φ ψ : Form} {v : SVAR} (p : ¬ is_free v φ):
+  | ax_q1 {Γ : set Form} {φ ψ : Form} {v : SVAR} (p : ¬ is_free v φ):
         Proof Γ ((all v, φ ⟶ ψ) ⟶ (φ ⟶ all v, ψ))
 
   -- two different instances of Axiom Q2: one for SVAR, one for NOM
-  | ax_q2_svar {φ : Form} (v : SVAR) (s : SVAR) (p : is_substable φ s v):
+  | ax_q2_svar {Γ : set Form} {φ : Form} (v : SVAR) (s : SVAR) (p : is_substable φ s v):
       Proof Γ ((all v, φ) ⟶ φ[s // v])
 
-  | ax_q2_nom  {φ ψ : Form} (v : SVAR) (s : NOM):
+  | ax_q2_nom  {Γ : set Form} {φ : Form} (v : SVAR) (s : NOM):
       Proof Γ ((all v, φ) ⟶ φ[s // v])
 
-  | ax_name (v : SVAR):
+  | ax_name {Γ : set Form} (v : SVAR):
       Proof Γ (ex v, v)
 
-  | ax_nom {φ : Form} {v : SVAR} (n m : Nat):
-      Proof Γ (iterate_pos n (φ ⋀ v) ⟶ iterate_nec m (v ⟶ φ))
+  | ax_nom {Γ : set Form} {φ : Form} {v : SVAR} (m n : Nat):
+      Proof Γ (all v, (iterate_pos m (v ⋀ φ) ⟶ iterate_nec n (v ⟶ φ)))
 
-  | ax_brcn {φ : Form} {v : SVAR}:
-      Proof Γ (all v, (□ φ) ⟶ (□ all v, φ))
+  | ax_brcn {Γ : set Form} {φ : Form} {v : SVAR}:
+      Proof Γ ((all v, □ φ) ⟶ (□ all v, φ))
 
 def Theorem {φ : Form} := ∀ Γ : set Form, Proof Γ φ  
 
