hybrid/README.md
@@ -4,33 +4,25 @@ Code was written following Blackburn 1998, present in this repository as **black
 
 - [What was done](#what-was-done)
 - [What needs work](#what-needs-work)
-  * [1. Substitution lemma](#1-substitution-lemma)
+  * [1. Soundness for tautologies & deduction rules](#1-soundness-for-tautologies-deduction-rules)
   * [2. Propositional tautologies](#2-propositional-tautologies)
-  * [3. Soundness for the remaining axioms](#3-soundness-for-the-remaining-axioms)
-  * [4. Proving decidability](#4-proving-decidability)
-  * [5. Completeness...](#5-completeness)
+  * [3. Completeness...](#5-completeness)
 - [In addition...](#in-addition)
 
 ### What was done
 1. Defined the basics of hybrid language (specifically the language L(∀) as per Blackburn 1998): **Form.lean**. Proved some basics facts about substitutions and boundness.
-2. Defined the proof system (but work is needed on propositional tautologies): **Proof.lean**.
+2. Defined the proof system: **Proof.lean**.
 3. Defined the semantics: **Truth.lean**. Proved some facts about interpretation variants and also that universal binding is commutative (semantically).
-4. Started working on soundness: **Soundness.lean**. Proved the correctness of axioms **K**, **Q1** and **Q2 for state variables**.
+4. Started working on soundness: **Soundness.lean**. Proved the correctness of axioms **K**, **Q1**, **Q2**, **Name**, **Nom** and **Barcan**, and also of **modus ponens**.
 
 ### What needs work
-#### 1. Substitution lemma
-Convince Lean that the proof for *svar_substitution:* (is_substable φ y x) → (is_variant g g' x) → (g' x = g y) → **((M,s,g) ⊨ φ[y // x] ↔ (M,s,g') ⊨ φ**) terminates. Well-founded induction was used in two places there:
-1. To prove the case for **φ = □ψ**, the induction hypothesis was applied to any neighbouring s' of s and to the formula ψ: **(M,s',g) ⊨ ψ[y // x] ↔ (M,s',g’) ⊨ ψ**.
-2. To prove the case for **φ = all v, ψ**, the induction hypothesis was applied to any v-variant f of g and to the formula ψ: **(M,s,f) ⊨ ψ[y // x] ↔ (M,s,f’) ⊨ ψ**.
+#### 1. Soundness for tautologies & deduction rules
+A proof of soundness for **propositional tautologies**, the **necessitation rule** and the **universalization rule** is still required. For the two rules, the proof is trivial if you decide to prove merely that (⊢ φ) → (⊨ φ). (As Blackburn does in his paper!) It gets harder if you insist on proving *strong* soundness: (Γ ⊢ φ) → (Γ ⊨ φ).
 
-Both of these applications seem sound to me. In both cases **ψ < φ** w.r.t. formula size, and in the end recursion should terminate when ψ becomes an atomic formula (size 1). I tried providing proofs that **ψ < □ψ** and **ψ < all v, ψ** via *have* statements. But that did nothing, because the actual goal that Lean wanted me to prove for termination was much, much uglier. The tactic state needed for termination is so long that I had to attach it in a separate file, *termination_state*. I don't know how to prove that.
 #### 2. Propositional tautologies
-Add an instance of every propositional tautology as an axiom and prove their soundness. I saw the way it was done in Matching Logic via morphisms, but I still have to wrap my head around it.
-#### 3. Soundness for the remaining axioms
-Namely **Q2 for nominals**, **Name**, Nom and **Barcan**, and the remaining deduction rules (modus ponens, generalization, necessitation). Proofs for bolded axioms can be found in Blackburn 1998.
-#### 4. Proving decidability
-I know this isn't *necessary* since I'm using Classical, but I want to at least be able to do it. I wanted to write an instance of Decidable for is_free x φ and I got stuck. I think I must provide a proof of either isTrue (is_free x φ) or isFalse (is_free x φ), but I don't know how to do that.
-#### 5. Completeness...
+This is not strictly necessary, but it would be nice to prove that the definition of tautologies via morphisms is equivalent to the usual definition by evaluations.
+
+#### 3. Completeness...
 
 ### In addition...
-Blackburn's paper proves ⊢φ ↔ ⊨φ, what I started proving is Γ⊢φ ↔ Γ⊨φ. That already means a bit more care is necessary when dealing with, e.g., the universal generalization axiom. I hope it won't become even more troublesome as I progress with the proof.
+Blackburn's paper proves ⊢φ ↔ ⊨φ, what I started proving is Γ⊢φ ↔ Γ⊨φ. That already means a bit more care is necessary when dealing with, e.g., the universal generalization axiom. A decision must be made regarding whether to proceed like this or revert to the weak soundness/completeness.
